%% !TEX TS-program = pdflatex
%% !TEX encoding = UTF-8 Unicode

\documentclass[12pt]{article} % use larger type; default would be 10pt

\usepackage[utf8]{inputenc} % set input encoding (not needed with XeLaTeX)

%%% Examples of Article customizations
% These packages are optional, depending whether you want the features they provide.
% See the LaTeX Companion or other references for full information.

%%% PAGE DIMENSIONS
\usepackage{geometry} % to change the page dimensions
\geometry{a4paper} % or letterpaper (US) or a5paper or....
\usepackage{setspace}
\usepackage{parskip}
\parskip=1\baselineskip %\advance\parskip by 0pt plus 2pt% to change between paragraphs space
% \geometry{margin=2in} % for example, change the margins to 2 inches all round
% \geometry{landscape} % set up the page for landscape
%   read geometry.pdf for detailed page layout information

% \usepackage{gravarphicx} % support the \includegravarphics command and options

% \usepackage[parfill]{parskip} % Activate to begin paragraphs with an empty line rather than an indent

%%% PACKAGES
\usepackage{booktabs} % for much better looking tables
\usepackage{array} % for better arrays (eg matrices) in maths
\usepackage{paralist} % very flexible & customisable lists (eg. enumerate/itemize, etc.)
\usepackage{verbatim} % adds environment for commenting out blocks of text & for better verbatim
\usepackage{subfig} % make it possible to include more than one captioned figure/table in a single float
% These packages are all incorporated in the memoir class to one degree or another...
\usepackage[fleqn]{amsmath}
\usepackage{amssymb}
\usepackage{enumitem}
\usepackage{amsthm}
\usepackage{graphicx}
\usepackage{filecontents}
\usepackage{natbib}
\usepackage{scrextend}
\usepackage[table,xcdraw]{xcolor}
\usepackage{tabularx}
% If you use beamer only pass "xcolor=table" option, i.e. \documentclass[xcolor=table]{beamer}
\usepackage{lscape}
\usepackage{longtable}
 \usepackage{booktabs}




%%% HEADERS & FOOTERS
\usepackage{fancyhdr} % This should be set AFTER setting up the page geometry
\pagestyle{fancy} % options: empty , plain , fancy
\renewcommand{\headrulewidth}{0pt} % customise the layout...
\lhead{}\chead{}\rhead{}
\lfoot{}\cfoot{\thepage}\rfoot{}

%%% SECTION TITLE APPEARANCE
\usepackage{sectsty}
\allsectionsfont{\rmfamily\bfseries\upshape} % (See the fntguide.pdf for font help)
% (This matches ConTeXt defaults)

%%% ToC (table of contents) APPEARANCE
\usepackage[nottoc,notlof,notlot]{tocbibind} % Put the bibliography in the ToC
\usepackage[titles,subfigure]{tocloft} % Alter the style of the Table of Contents
\renewcommand{\cftsecfont}{\rmfamily\mdseries\upshape}
\renewcommand{\cftsecpagefont}{\rmfamily\mdseries\upshape} % No bold!

\usepackage[colorlinks,citecolor=black,urlcolor=black,bookmarks=false,hypertexnames=true]{hyperref} 
%%% END Article customizations
%%% The "real" document content comes below...

\title{Solution Akcigit Ates JPE 2023}
\author{Xing Mingjie 3036029301}
\date{\today} % Activate to display a given date or no date (if empty),
         % otherwise the current date is printed 

\begin{document}
\maketitle

\section{Consumer}

Consumer solves 
\[\begin{equation}
	V_t = \mathop{max}\limits_{C_s} \int_t^\infty \exp{(-\rho(s-t))}\ln C_s \, ds
\end{equation}\]

subject to $\dot{A_t} = w_t L_t + r_t A_t + G_t - P_t C_t$.

The Bellman reads 

\[\begin{equation}
	\rho V(A_t) = \mathop{max}\limits_{C_t} \ln C_t + V^\prime(A_{t}) \dot{A_t}
\end{equation}\]

Take derivate w.r.t. $C_t$ gives
\[0 = \frac{1}{C_t} - V^\prime(A_t) P_t\]
So we have 
\[C_t = P_t^{-1}V^\prime (A_t)^{-1}\]

And the Envelope theorem
\[\begin{aligned}
	(\rho-r_t) V^\prime(A_t) &= V^{\prime\prime}(A_t)\dot{A_t}\\
	(\rho-r_t) (P_t C_t)^{-1} &= -P_t^{-1} C_t^{-2} \frac{dC_t}{dA_t} \frac{dA_t}{dt}\\
	\frac{\dot{C_t}}{C_t} & = r_t - \rho\\
	r_t &= \rho + g_t\\
\end{aligned}\]
where $g_t = \frac{\dot{C_t}}{C_t}$ and $V^{\prime\prime}(A_t) = -P_t^{-1}C_t^{-2}C_t^\prime$.

\section{Final Producer}

Final producer solves
\[\begin{equation*}
	\mathop{max}\limits_{y_{jt}} P_t Y_t - \int_0^1 p_{jt} y_{jt} \, dj\\
	\text{subject to} \ln{Y_t} = \int_0^1 \ln y_{jt} \, dj
\end{equation*}\]

The marginal profit of the Final producer should equal the marginal cost:
\[\begin{align}
	\frac{\partial P_t Y_t}{\partial y_{jt}} &= p_{jt}\\
	\Rightarrow
	P_t \times \exp{(\int_0^1 \ln y_{jt} \,dj)} \times \frac{1}{y_{jt}} &= p_{jt}\\
	\Rightarrow
	P_t Y_t &= p_{jt}y_{jt}\\
	\Rightarrow
	\ln Y_t &= \int^1_0 \ln \frac{P_tY_t}{p_{jt}}\, dj\\
		&= \ln P_tY_t - \int^1_0 \ln p_{jt}\, dj\\
\end{align}\]
\[\begin{equation}
	\Leftrightarrow
	lnP_t = \int^1_0 \ln p_{jt}\, dj\\
\end{equation}\]
which is the optimal demand.

\section{Sectoral intermediate production}
On sectoral level, the intermediate production's optimal supply of products solves

\[
	\mathop{max}\limits_{y_{ijt},y_{-ijt}} P_{jt} Y_{jt} - (p_{ijt}y_{ijt}+p_{-ijt}y_{-ijt})\\
	\text{subject to } Y_{jt} = (y_{ijt}^\beta +y_{-ijt}^\beta)^{1/ \beta}
\]

Setting marginal cost and product equal yields
\[\begin{align}
	P_{jt} \frac{\partial Y_{jt}}{\partial y_{ijt}} = p_{ijt}\\
	P_{jt} \frac{1}{\beta} (y_{ijt}^\beta +y_{-ijt}^\beta)^\frac{1-\beta}{\beta} \cdot \beta y_{ijt}^{\beta-1}=p_{ijt}\\
	y_{ijt} = (\frac{p_{ijt}}{P_{jt}})^\frac{1}{\beta-1}\cdot Y_{jt}
\end{align}\]
Symmetry gives
\[
y_{-ijt} = (\frac{p_{-ijt}}{P_{jt}})^\frac{1}{\beta-1}\cdot Y_{jt}
\]
Substituting into sectoral constraint gives 
\[
	Y_{jt} = ((\frac{p_{ijt}}{P_{jt}})^\frac{\beta}{\beta-1}+(\frac{p_{-ijt}}{P_{jt}})^\frac{\beta}{\beta-1})^{1/\beta} Y_{jt}\\
\]
This gives the expression of $P_{jt}$

\[\begin{equation}
	P_{jt} = (p_{ijt}^\frac{\beta}{\beta-1}+p_{-ijt}^\frac{\beta}{\beta-1})^\frac{\beta-1}{\beta}
\end{equation}\]

And we combine with the firm level production and the fact that $P_t Y_t = p_{jt} y_{jt}$
\[\begin{equation}
	y_{ijt} = \frac{p_{ijt}^{\frac{1}{\beta-1}}}{p_{ijt}^\frac{\beta}{\beta-1}+p_{-ijt}^\frac{\beta}{\beta-1}} Y_t
\end{equation}\] 

The market share is given by
\[\begin{equation}
	z_{ijt} = \frac{p_{ijt}y_{ijt}}{Y_t} = \frac{p_{ijt}^{\frac{\beta}{\beta-1}}}{p_{ijt}^\frac{\beta}{\beta-1}+p_{-ijt}^\frac{\beta}{\beta-1}}
\end{equation}\]

\section{Firm Production}
Firm maximizes its profit by choosing price and production
\[\begin{equation}
	\pi_{ijt} = \max_{y_{ijt},p_{ijt}} (p_{ijt}-mc_{ijt})y_{ijt}\\
\end{equation}\]\\
Taking derivative of $p_{ijt}$
\[\begin{align*}
	y_{ijt} +(p_{ijt}-mc_{ijt})\frac{dy_{ijt}}{dp_{ijt}} = 0\\
	\frac{p_{ijt}^{\frac{1}{\beta-1}}}{p_{ijt}^\frac{\beta}{\beta-1}+p_{-ijt}^\frac{\beta}{\beta-1}} Y_t
	+ (p_{ijt}-mc_{ijt})\frac{\frac{1}{\beta-1}p_{ijt}^\frac{2-\beta}{\beta-1}-p_{ijt}^\frac{1}{\beta-1}\frac{\beta}{\beta-1}p_{ijt}^\frac{1}{\beta-1}}{(p_{ijt}^\frac{\beta}{\beta-1}+p_{-ijt}^\frac{\beta}{\beta-1})^2} Y_t = 0\\
\end{align*}\]
Making use of the definition of $z_{ijt}$ gives
\[
	(\beta-1)p_{ijt} + (p_{ijt}-mc_{ijt})(1-\beta z_{ijt})=0\\
\]
We yield
\[\begin{equation}
	p_{ijt} = \frac{1-\beta z_{ijt}}{\beta(1-z_{ijt})}mc_{ijt}
\end{equation}\]\\
We derive
\[\begin{aligned}
	\frac{p_{-ijt}}{p_{ijt}} &= \frac{1-\beta z_{-ijt}}{1-\beta z_{ijt}} \frac{\beta(1-z_{ijt})}{\beta(1-z_{-ijt})} \frac{q_{ijt}}{q_{-ijt}}\\
	&=\Xi(z_{ijt})\lambda^{\mathbb{F}(m_{ijt})}\\
	&=\Xi(z_{ijt})\lambda^m_{ijt}
\end{aligned}\]\\

Suppressing $j$ and we have the labour demand
\[\begin{aligned}
	l(m_{it}) &= \frac{y_{it}}{q_{it}}\\
	&= q_{it}^{-1}\frac{z_{it}}{p_{it}}Y_t\\
	&= \frac{z_{it}}{w_{it}}\frac{\beta(1-z_{it})}{1-\beta z_{it}} Y_t\\
	&= \omega_t^{-1} z_it \frac{\beta(1-z_{it})}{1-\beta z_{it}}\\
\end{aligned}\]\\

where $\omega_t = \frac{Y_t}{w_t}$ is the proportion of labor wage in the economy.

The profit
\[\begin{aligned}
	\pi (m_{it}) &= (p_{it}-mc_{it})y_{it}\\
	&= \frac{(1-\beta)z_{it}}{1-\beta z_{it}}Y_t\\
\end{aligned}\]

And markup
\[\begin{aligned}
	mu(m_{it}) &= \frac{p_{it}}{mc_{it}}-1\\
	&= \frac{1-\beta}{\beta(1-z_{it})}\\
\end{aligned}\]

And finally the elasticity of price
\[\begin{aligned}
	\varepsilon_{ijt} &= \frac{\partial \ln y_{ijt}}{\partial \ln p_{ijt}}\\
	&= \frac{\partial}{\partial\ln p_{ijt}} (\frac{1}{\beta-1}\ln p_{ijt}-\ln(p_{ijt}^\frac{\beta}{\beta-1}+p_{-ijt}^\frac{\beta}{\beta-1})+\ln Y_t)\\
	&= \frac{1-\beta z_{ijt}}{\beta-1} 
\end{aligned}\]


\footnotesize
\bibliographystyle{apalike}
%\bibliography{RP}


\end{document}
